ast: Refine definition of entities

src/AST/Entities.dfy
@@ -5,7 +5,7 @@ include "Names.dfy"
 include "Syntax.dfy"
 include "../Utils/Library.dfy"
 
-module Bootstrap.AST.Entities
+module {:options "-functionSyntax:4"} Bootstrap.AST.Entities
   // Hierarchies of Dafny entities.
   // See </doc/design/entities.md>.
 {
@@ -47,37 +47,151 @@ module Bootstrap.AST.Entities
     | DataType(dt: DataType)
     | NewType(nt: NewType)
 
+  datatype FieldKind =
+    Const | Var
   datatype Field =
-    | Field(tp: Type)
+    Field(kind: FieldKind, body: Expr)
 
-  datatype FuncKind =
-    Method | Function | Constructor
-  datatype Func =
-    | Func(kind: FuncKind, body: Expr)
+  datatype Callable =
+    | Method(body: Expr)
+    | Function(body: Expr)
+    | Constructor(body: Expr)
 
-  datatype RawEntity =
-    | Module(children: seq<Name>)
-    | ExportSet(provided: set<Name>, revealed: set<Name>)
-    | Import(localName: Atom, target: Name)
-    | Type(children: seq<Name>)
-    | Definition()
+  datatype Definition =
+    | Field(fi: Field)
+    | Callable(ci: Callable)
 
-  datatype Attribute =
-    Attribute(name: string, value: Expr)
+  datatype EntityKind =
+    | EModule
+    | EExportSet
+    | EImport
+    | EType
+    | EDefinition
+
+  type EntityInfo = e: EntityInfo_ | e.Valid?()
+    witness EntityInfo(Anonymous, attrs := [], members := [])
+  datatype EntityInfo_ =
+    EntityInfo(name: Name, nameonly attrs: seq<Attribute>, nameonly members: seq<Name>)
+  {
+    ghost predicate Valid?() {
+      forall nm <- members :: nm.ChildOf(name)
+    }
+  }
 
   datatype Entity =
-    Entity(e: RawEntity, attrs: seq<Attribute>, children: seq<Name>)
+    | Module(ei: EntityInfo)
+    | ExportSet(ei: EntityInfo, e: ExportSet)
+    | Import(ei: EntityInfo, i: Import)
+    | Type(ei: EntityInfo, t: Type)
+    | Definition(ei: EntityInfo, d: Definition)
+  {
+    const kind :=
+      match this
+        case Module(ei) => EModule
+        case ExportSet(ei, e) => EExportSet
+        case Import(ei, i) => EImport
+        case Type(ei, t) => EType
+        case Definition(ei, d) => EDefinition
+  }
 
-  datatype NamedEntity =
-    NamedEntity(n: Name, e: Entity)
+  datatype Attribute = // TODO: Move all exprs to top level?
+    Attribute(name: string, args: seq<Expr>)
+  {
+    function ToString(): string {
+      "{:" + name + (if args != [] then " ..." else "") + "}"
+    }
+  }
 
-  datatype Registry = Registry(entities: map<Name, Entity>) {
-    function method Find(n: Name) : Option<Entity> {
+  ghost predicate EntityMap?(f: Entity -> Entity) {
+    forall e ::
+      && f(e).kind == e.kind
+      && f(e).ei.name == e.ei.name
+      && f(e).ei.members == e.ei.members
+  }
+
+  type EntityMap = f | EntityMap?(f) witness e => e
+
+  type Registry = r: Registry_ | r.Valid?()
+    witness Registry(map[])
+  datatype Registry_ = Registry(entities: map<Name, Entity>)
+    // A collection of Dafny entities, index by name.
+    //
+    // The entity graph of a Dafny program is a tree: members of a module or
+    // class have names that extend that of the parent module.  This fact allows
+    // easy recursion, using the functions `SuffixesOf` and `SuffixesOfMany`
+    // below, along with the two recursion lemmas `Decreases_SuffixesOf` and
+    // `Decreases_SuffixesOfMany`.
+  {
+    ghost predicate ValidNames?() {
+      forall n <- entities :: entities[n].ei.name == n
+    }
+
+    ghost predicate ValidParent??(n: Name) {
+      n == Anonymous || n.parent in entities
+    }
+
+    ghost predicate ValidParents?() {
+      forall n <- entities :: ValidParent??(n)
+    }
+
+    ghost predicate ValidMembers??(ei: EntityInfo) {
+      forall m <- ei.members :: m in entities
+    }
+
+    ghost predicate ValidMembers?() {
+      forall n <- entities :: ValidMembers??(entities[n].ei)
+    }
+
+    ghost predicate Valid?() {
+      && ValidNames?()
+      && ValidParents?()
+      && ValidMembers?()
+    }
+
+    ghost function {:opaque} SuffixesOf(name: Name): set<Name> {
+      set n <- entities | n.SuffixOf(name)
+    }
+
+    ghost function {:opaque} SuffixesOfMany(names: seq<Name>): set<Name> {
+      set n <- names, sf <- SuffixesOf(n) :: sf
+    }
+
+    lemma Decreases_SuffixesOfMany(ei: EntityInfo)
+      requires ei.name in entities
+      ensures SuffixesOfMany(ei.members) < SuffixesOf(ei.name);
+    {
+      reveal SuffixesOf();
+      reveal SuffixesOfMany();
+
+      assert SuffixesOfMany(ei.members) <= SuffixesOf(ei.name) by {
+        forall sf <- SuffixesOfMany(ei.members)
+          ensures sf in SuffixesOf(ei.name)
+        {
+          var name: Name :| name in ei.members && sf in SuffixesOf(name);
+          Name.SuffixOf_Transitive(ei.name, name, sf);
+        }
+      }
+
+      assert ei.name in SuffixesOf(ei.name);
+      assert ei.name !in SuffixesOfMany(ei.members);
+    }
+
+    lemma {:induction false} Decreases_SuffixesOf(names: seq<Name>, name: Name)
+      requires name in names
+      ensures SuffixesOf(name) <= SuffixesOfMany(names);
+    {
+      reveal SuffixesOf();
+      reveal SuffixesOfMany();
+    }
+
+    function Find(n: Name) : Option<Entity> {
       if n in entities then Some(entities[n]) else None
     }
 
-    function method Map(f: NamedEntity -> Entity) : Registry {
-      Registry(map n | n in entities :: f(NamedEntity(n, entities[n])))
+    function Map(f: EntityMap) : Registry
+      requires Valid?()
+    {
+      Registry(map n | n in entities :: f(entities[n]))
     }
   }
 }
