src/AST/Names.dfy
@@ -1,4 +1,4 @@
-module Bootstrap.AST.Names {
+module {:options "-functionSyntax:4"} Bootstrap.AST.Names {
   type Atom =
     // An individual component of a Dafny name.
     s: string | s != "" && '.' !in s witness "n"
@@ -7,10 +7,59 @@ module Bootstrap.AST.Names {
     | Anonymous
     | Name(parent: Name, suffix: Atom)
   {
-    predicate method Extends(parent: Name)
-      // Check whether `this` is a descendant of `parent`.
+    function Length(): nat {
+      match this
+        case Anonymous => 0
+        case Name(_, _) => 1 + parent.Length()
+    }
+
+    function ToString(): string {
+      match this
+        case Anonymous => "_"
+        case Name(Anonymous, suffix) => suffix
+        case Name(parent, suffix) => parent.ToString() + "." + suffix
+    }
+
+    predicate ChildOf(parent: Name)
+      // Check whether `this` is a direct descendant of `parent`.
+      ensures ChildOf(parent) ==> Length() == parent.Length() + 1
     {
-      this.Name? && this.parent == parent
+      this.Name? && parent == this.parent
+    }
+
+    predicate StrictSuffixOf(parent: Name)
+      // Check whether one of the parents of `this` is `parent`.
+      ensures StrictSuffixOf(parent) ==> Length() > parent.Length()
+    {
+      this != parent && SuffixOf(parent)
+    }
+
+    predicate SuffixOf(parent: Name)
+      // Check whether `this` descended from `parent`.
+      decreases this
+      ensures SuffixOf(parent) ==> Length() >= parent.Length()
+    {
+      || parent == this
+      || (this.Name? && this.parent.SuffixOf(parent))
+    }
+
+    static lemma {:induction n2} SuffixOf_Transitive(n0: Name, n1: Name, n2: Name)
+      requires n2.SuffixOf(n1) && n1.SuffixOf(n0)
+      ensures n2.SuffixOf(n0)
+    {}
+
+    static lemma {:induction false} StrictSuffixOf_Left_Transitive(n0: Name, n1: Name, n2: Name)
+      requires n2.StrictSuffixOf(n1) && n1.SuffixOf(n0)
+      ensures n2.StrictSuffixOf(n0)
+    {
+      SuffixOf_Transitive(n0, n1, n2);
+    }
+
+    static lemma {:induction false} StrictSuffixOf_Right_Transitive(n0: Name, n1: Name, n2: Name)
+      requires n2.SuffixOf(n1) && n1.StrictSuffixOf(n0)
+      ensures n2.StrictSuffixOf(n0)
+    {
+      SuffixOf_Transitive(n0, n1, n2);
     }
   }
 }
